src/program_proof/mvcc/txn_abort.v
@@ -1,27 +1,58 @@
-From Perennial.program_proof.mvcc Require Import txn_common txnmgr_deactivate.
+From Perennial.program_proof.mvcc Require Import proph_proof txn_common txnmgr_deactivate.
 
 Section program.
 Context `{!heapGS Σ, !mvcc_ghostG Σ}.
 
-Theorem wp_txn__Abort_false txn tid tmods γ τ :
-  {{{ own_txn txn tid γ τ ∗ cmt_tmods_frag γ tmods }}}
+Definition abort_false_cases γ : iProp Σ :=
+  (∃ tid, nca_tids_frag γ tid) ∨
+  (∃ tmods, fci_tmods_frag γ tmods) ∨
+  (∃ tmods, fcc_tmods_frag γ tmods) ∨
+  (∃ tmods, cmt_tmods_frag γ tmods).
+
+Theorem wp_txn__Abort_false txn tid γ τ :
+  {{{ own_txn txn tid γ τ ∗ abort_false_cases γ }}}
     Txn__Abort #txn
   {{{ RET #(); False }}}.
 Admitted.
 
 Theorem wp_txn__Abort txn tid γ τ :
-  {{{ own_txn txn tid γ τ }}}
+  {{{ own_txn txn tid γ τ ∗ fa_tids_frag γ tid }}}
     Txn__Abort #txn
   {{{ RET #(); own_txn_uninit txn γ }}}.
 Proof.
-  iIntros (Φ) "Htxn HΦ".
+  iIntros (Φ) "[Htxn Hfrag] HΦ".
   wp_call.
+
+  (***********************************************************)
+  (* proph.ResolveAbort(txn.txnMgr.p, txn.tid)               *)
+  (***********************************************************)
+  iNamed "Htxn".
+  iNamed "Himpl".
+  do 3 wp_loadField.
+  wp_apply (wp_ResolveAbort); first auto.
+  iInv "Hinv" as "> HinvO" "HinvC".
+  iApply ncfupd_mask_intro; first set_solver.
+  iIntros "Hclose".
+  iNamed "HinvO".
+  iExists future.
+  iFrame "Hproph".
+  iIntros "(%future' & %Hhead & Hproph)".
+  iMod "Hclose" as "_".
+  (* Update the sets of ok/doomed txns to re-establish inv w.r.t. [future']. *)
+  iDestruct (nca_inv_any_action with "Hnca") as "Hnca"; first apply Hhead.
+  iMod (fa_inv_same_action with "Hfrag Hfa") as "Hfa"; first apply Hhead.
+  iDestruct (fci_inv_diff_action with "Hfci") as "Hfci"; [apply Hhead | done |].
+  iDestruct (fcc_inv_diff_action with "Hfcc") as "Hfcc"; [apply Hhead | done |].
+  iDestruct (cmt_inv_diff_action with "Hcmt") as "Hcmt"; [apply Hhead | done |].
+  iDestruct (per_key_inv_past_abort tid with "Hkeys") as "Hkeys".
+  iMod ("HinvC" with "[- HΦ Htid Hsid Hwrbuf HwrbufRP Hactive Hltuples Htxnmap]") as "_".
+  { (* Close the invariant. *) eauto 15 with iFrame. }
+  iIntros "!> _".
+  wp_pures.
 
   (***********************************************************)
   (* txn.txnMgr.deactivate(txn.sid, txn.tid)                 *)
   (***********************************************************)
-  iNamed "Htxn".
-  iNamed "Himpl".
   do 3 wp_loadField.
   wp_apply (wp_txnMgr__deactivate with "HtxnmgrRI Hactive").
   wp_pures.
@@ -30,3 +61,5 @@ Proof.
 Qed.
 
 End program.
+
+Hint Extern 1 (environments.envs_entails _ (abort_false_cases _)) => unfold abort_false_cases : core.
