src/program_proof/mvcc/txn_commit.v
@@ -3,22 +3,25 @@ From Perennial.program_proof.mvcc Require Import txn_common.
 Section program.
 Context `{!heapGS Σ, !mvcc_ghostG Σ}.
 
-Definition abort_cases γ : iProp Σ :=
+(* TODO: the last case also needs [¬ Q r w].*)
+Definition commit_false_cases γ : iProp Σ :=
   (∃ tid, nca_tids_frag γ tid) ∨
   (∃ tid, fa_tids_frag γ tid)  ∨
-  (∃ tmod, fci_tmods_frag γ tmod) ∨
-  (∃ tmod, fcc_tmods_frag γ tmod).
+  (∃ tmods, fci_tmods_frag γ tmods) ∨
+  (∃ tmods, fcc_tmods_frag γ tmods).
 
 Theorem wp_txn__Commit_false txn tid γ τ :
-  {{{ own_txn_ready txn tid γ τ ∗ abort_cases γ }}}
+  {{{ own_txn_ready txn tid γ τ ∗ commit_false_cases γ }}}
     Txn__Commit #txn
   {{{ (ok : bool), RET #ok; False }}}.
 Admitted.
 
-Theorem wp_txn__Commit txn tid γ τ :
-  {{{ own_txn_ready txn tid γ τ }}}
+Theorem wp_txn__Commit txn tid tmods γ τ :
+  {{{ own_txn_ready txn tid γ τ ∗ cmt_tmods_frag γ tmods }}}
     Txn__Commit #txn
   {{{ (ok : bool), RET #ok; own_txn_uninit txn γ }}}.
 Admitted.
 
 End program.
+
+Hint Extern 1 (environments.envs_entails _ (commit_false_cases _)) => unfold commit_false_cases : core.
